progress on proving the poly_equivalence lemma

code/experimental/ctr-poly-vec/Hacl.Poly.Equiv.fst
@@ -9,6 +9,7 @@ open Hacl.Poly
 
 #set-options "--z3rlimit 50 --max_fuel 0 --max_ifuel 0"
 
+module Loops = Lib.LoopCombinators
 
 //TODO: change the definition of the repeat_blocks function in Lib.Sequence
 val repeat_blocks_split:
@@ -32,6 +33,45 @@ val repeat_blocks_split:
 let repeat_blocks_split #a #b #c blocksize len0 inp f l acc0 = admit()
 
 
+val repeat_blocks_last:
+    #w:lanes
+  -> text:bytes{length text < w * blocksize}
+  -> acc_v:felem_v w
+  -> r:felem -> Lemma
+  (let pre = create w (pow_w w r) in
+   repeat_blocks #uint8 #(felem_v w) #felem (w * blocksize) text (poly_update_nblocks #w pre) (poly_update_last_v #w r) acc_v ==
+   poly_update_last_v #w r (length text) text acc_v)
+
+let repeat_blocks_last #w text acc_v r =
+  let pre = create w (pow_w w r) in
+  let len = length text in
+  let blocksize_v = w * blocksize in
+  let nb = len / blocksize_v in
+  Math.Lemmas.small_div len blocksize_v;
+  assert (nb = 0);
+  let rem = len % blocksize_v in
+  let acc = Loops.repeati nb (repeat_blocks_f (w * blocksize) text (poly_update_nblocks #w pre) nb) acc_v in
+  Loops.eq_repeati0 nb (repeat_blocks_f (w * blocksize) text (poly_update_nblocks #w pre) nb) acc_v;
+  assert (acc == acc_v);
+  let last = Seq.slice text (nb * blocksize_v) len in
+  Seq.Properties.slice_length text
+
+
+val repeat_blocks_multi_v_equiv:
+    #w:lanes
+  -> text:bytes{length text % (w * blocksize) = 0}
+  -> acc_v0:felem_v w
+  -> r:felem -> Lemma
+  (let pre = create w (pow_w w r) in
+   Math.Lemmas.mod_mult_exact (length text) blocksize w;
+   normalize_v r (repeat_blocks_multi (w * blocksize) text (poly_update_nblocks #w pre) acc_v0) ==
+   repeat_blocks_multi blocksize text (poly_update1 r) (normalize_v r acc_v0))
+
+let repeat_blocks_multi_v_equiv #w text acc_v0 r = admit()
+
+
+
+
 val repeat_blocks_v_equiv:
     #w:lanes
   -> text:bytes
@@ -41,10 +81,27 @@ val repeat_blocks_v_equiv:
    repeat_blocks #uint8 #(felem_v w) #felem (w * blocksize) text (poly_update_nblocks #w pre) (poly_update_last_v #w r) acc_v0 ==
    repeat_blocks #uint8 #felem #felem blocksize text (poly_update1 r) (poly_update_last r) (normalize_v r acc_v0))
 
-let repeat_blocks_v_equiv #w text acc_v0 r = admit()
-// call `repeat_blocks_split` with len0 = len / bs_v * bs_v [f_v; [f; g]]
-// repeat_blocks_multi (v == s) [f; [f; g]]
-// call `repeat_blocks_multi_split` [f; g]
+let repeat_blocks_v_equiv #w text acc_v0 r =
+  let blocksize_v = w * blocksize in
+  let len = length text in
+  let len0 = len / blocksize_v * blocksize_v in
+  FStar.Math.Lemmas.cancel_mul_mod (len / blocksize_v) blocksize_v;
+  assert (len0 % blocksize_v = 0);
+
+  let pre = create w (pow_w w r) in
+  let acc = repeat_blocks #uint8 #(felem_v w) #felem blocksize_v text (poly_update_nblocks #w pre) (poly_update_last_v #w r) acc_v0 in
+  repeat_blocks_split #uint8 #(felem_v w) #felem blocksize_v len0 text (poly_update_nblocks #w pre) (poly_update_last_v #w r) acc_v0;
+  let acc_v1 = repeat_blocks_multi blocksize_v (Seq.slice text 0 len0) (poly_update_nblocks #w pre) acc_v0 in
+  repeat_blocks_last #w (Seq.slice text len0 len) acc_v1 r;
+  assert (acc == poly_update_last_v #w r (len - len0) (Seq.slice text len0 len) acc_v1);
+  assert (acc == poly_update (Seq.slice text len0 len) (normalize_v r acc_v1) r);
+  assert (acc == repeat_blocks #uint8 #felem blocksize (Seq.slice text len0 len) (poly_update1 r) (poly_update_last r) (normalize_v r acc_v1));
+  repeat_blocks_multi_v_equiv #w (Seq.slice text 0 len0) acc_v0 r;
+
+  Math.Lemmas.paren_mul_right (len / blocksize_v) w blocksize;
+  Math.Lemmas.cancel_mul_mod (len / blocksize_v * w) blocksize;
+  assert (len0 % blocksize = 0);
+  repeat_blocks_split #uint8 #felem blocksize len0 text (poly_update1 r) (poly_update_last r) (normalize_v r acc_v0)
 
 
 let poly_equivalence #w text acc0 r =
